Clean/Ironwood/NoteCommit/Composites.lean
@@ -102,11 +102,12 @@ def circuit :
 
   synthesize := fun (gcfg, lcfg) input => synth gcfg lcfg input
 
-  elaborated := fun (gcfg, lcfg) =>
-    { output := fun _ _ => ()
-      regionCount := fun _ => 2
-      output_eq := by intro _ _; rfl
-      regionCount_eq := fun input i => (synth_regionCount gcfg lcfg input i).symm }
+  elaborated :=
+    { output := fun _ _ _ => ()
+      regionCount _ := 2
+      output_eq := by intro _ _ _; rfl
+      regionCount_eq := fun (gcfg, lcfg) input i =>
+        (synth_regionCount gcfg lcfg input i).symm }
 
   EnvAssumptions := fun (_, lcfg) env =>
     LookupRangeCheck.TableLoaded 10 lcfg env.env ∧
@@ -250,11 +251,12 @@ def circuit :
 
   synthesize := fun (gcfg, lcfg) input => synth gcfg lcfg input
 
-  elaborated := fun (gcfg, lcfg) =>
-    { output := fun _ _ => ()
-      regionCount := fun _ => 2
-      output_eq := by intro _ _; rfl
-      regionCount_eq := fun input i => (synth_regionCount gcfg lcfg input i).symm }
+  elaborated :=
+    { output := fun _ _ _ => ()
+      regionCount _ := 2
+      output_eq := by intro _ _ _; rfl
+      regionCount_eq := fun (gcfg, lcfg) input i =>
+        (synth_regionCount gcfg lcfg input i).symm }
 
   EnvAssumptions := fun (_, lcfg) env =>
     LookupRangeCheck.TableLoaded 10 lcfg env.env ∧
@@ -391,11 +393,12 @@ def circuit :
 
   synthesize := fun (gcfg, lcfg) input => synth gcfg lcfg input
 
-  elaborated := fun (gcfg, lcfg) =>
-    { output := fun _ _ => ()
-      regionCount := fun _ => 2
-      output_eq := by intro _ _; rfl
-      regionCount_eq := fun input i => (synth_regionCount gcfg lcfg input i).symm }
+  elaborated :=
+    { output := fun _ _ _ => ()
+      regionCount _ := 2
+      output_eq := by intro _ _ _; rfl
+      regionCount_eq := fun (gcfg, lcfg) input i =>
+        (synth_regionCount gcfg lcfg input i).symm }
 
   EnvAssumptions := fun (_, lcfg) env =>
     LookupRangeCheck.TableLoaded 10 lcfg env.env ∧
@@ -533,11 +536,12 @@ def circuit :
 
   synthesize := fun (gcfg, lcfg) input => synth gcfg lcfg input
 
-  elaborated := fun (gcfg, lcfg) =>
-    { output := fun _ _ => ()
-      regionCount := fun _ => 2
-      output_eq := by intro _ _; rfl
-      regionCount_eq := fun input i => (synth_regionCount gcfg lcfg input i).symm }
+  elaborated :=
+    { output := fun _ _ _ => ()
+      regionCount _ := 2
+      output_eq := by intro _ _ _; rfl
+      regionCount_eq := fun (gcfg, lcfg) input i =>
+        (synth_regionCount gcfg lcfg input i).symm }
 
   EnvAssumptions := fun (_, lcfg) env =>
     LookupRangeCheck.TableLoaded 10 lcfg env.env ∧
